Forwarding_Code.eca should have been using UCBasicTypes.ec, but the latter thus needed to define addr, mode and msg (which were in UCCore.ec). So now the UC DSL typechecker issues a warning message if these types and associated constructors and operators are defined in .ec files ec_required by a UC DSL spec - as this isn't useful, and may result in different definitions being in scope in the generated EasyCrypt code.
(KeyExchange is in progress.)

uc-dsl/src/ucSpec.ml
@@ -28,6 +28,8 @@ let parse_error = error_message
 
 let type_error = error_message
 
+let type_warning = warning_message
+
 (* symbols *)
 
 let qsymb_of_symb (x : symbol) : qsymbol = ([], x)
@@ -249,7 +251,8 @@ type def =
 
 (* UC and EasyCrypt requires *)
 
-type externals = {uc_requires : psymbol list; ec_requires : psymbol list}
+type externals =
+  {uc_requires : psymbol list; ec_requires : psymbol list}
 
 (* overall UC specifications *)
 
