common/UCBasicTypes.ec
@@ -1,10 +1,14 @@
 (* UCBasicTypes.ec *)
 
 (* Defines encoding and partial decoding pairs (EPDPs), the type
-   univ plus a number of EPDPs with target univ, addresses
-   and ports *)
+   univ plus a number of EPDPs with target univ, addresses,
+   ports and messages *)
 
 require import AllCore List.
+
+(* prefix ordering on lists *)
+
+require import UCListPO.  (* only needed to define envport, below *)
 
 (* defines encoding and partial decoding pairs (EPDPs) *)
 
@@ -20,7 +24,7 @@ require export UCUniv.
 
    if a functionality has address alpha, it is also responsible for all
    sub-functionalities with addresses beta >= alpha (in the prefix
-   partial ordering of UCListPO)
+   partial ordering)
 
    adversaries are also modeled as functionalities - but with no
    sub-addresses/sub-functionalties; simulators are functionalities
@@ -28,13 +32,13 @@ require export UCUniv.
 
    [] is the root address of the environment *)
 
-type _addr = int list.  (* begins with _, as not exposed to UC DSL *)
+type addr = int list.
 
-op epdp_addr_univ : (_addr, univ) epdp = epdp_list_univ epdp_int_univ.
+op epdp_addr_univ : (addr, univ) epdp = epdp_list_univ epdp_int_univ.
 
 lemma valid_epdp_addr_univ : valid_epdp epdp_addr_univ.
 proof.
-rewrite valid_epdp_list_univ valid_epdp_int_univ.
+rewrite epdp_sub epdp.
 qed.
 
 hint simplify [eqtrue] valid_epdp_addr_univ.
@@ -49,15 +53,53 @@ hint rewrite epdp : valid_epdp_addr_univ.
 
    ([], 0) is the root port of the environment *)
 
-type port = _addr * int.
+type port = addr * int.
 
 op epdp_port_univ : (port, univ) epdp =
-  epdp_pair_univ epdp_addr_univ epdp_int_univ.
+  epdp_pair_univ (epdp_list_univ epdp_int_univ) epdp_int_univ.
 
 lemma valid_epdp_port_univ : valid_epdp epdp_port_univ.
 proof.
-rewrite epdp_sub epdp.
+rewrite !epdp_sub epdp.
 qed.
 
 hint simplify [eqtrue] valid_epdp_port_univ.
 hint rewrite epdp : valid_epdp_port_univ.
+
+(* in UC DSL, envport is a keyword, and so cannot be used as an
+   ordinary identifier. in DSL specs, it has type port -> bool, but in
+   the generated EasyCrypt code it has type _addr -> addr -> bool, and
+   is applied to the address of the functionality and adversary - in
+   addition to the port expression *)
+
+op envport (self adv : addr, pt : port) : bool =
+  ! self <= pt.`1 /\ ! adv <= pt.`1  /\ pt <> ([], 0).
+
+(* messages have modes:
+
+     * direct - supplying functionality inputs, consuming their
+         outputs
+
+     * adversarial - communication between functionalties and
+         adversaries/simulators, communication between different
+         adversaries/simulators, and communication between
+         environments and adversaries/simulators *)
+
+type mode = [
+  | Dir  (* direct *)
+  | Adv  (* adversarial *)
+].
+
+lemma not_dir (mod : mode) :
+  mod <> Dir <=> mod = Adv.
+proof. by case mod. qed.
+
+lemma not_adv (mod : mode) :
+  mod <> Adv <=> mod = Dir.
+proof. by case mod. qed.
+
+(* a message has the form (mod, pt1, pt2, tag, u), for a mode mod, a
+   destination port pt1, a source port pt2, an integer tag (used to
+   ensure certain messages are distinct), and a universe value u *)
+
+type msg = mode * port * port * int * univ.
