uc-dsl/examples/smc-case-study/Forwarding.uc
@@ -1,6 +1,6 @@
 (* Forwarding *)
 
-ec_requires KeysExponentsAndPlainTexts.
+ec_requires KeysExponentsAndPlaintexts.
 
 direct FwDir_ {
   in pt1@fw_req(pt2 : port, u : univ)
