uc-dsl/prelude/README.md
@@ -8,5 +8,5 @@ and `.uc` files.
 The files `UCEncoding.ec` and `UCUniv.ec` are symbolic links to those files
 in `../Common`.
 
-The file `UCBasicTypes.ec` is a more abstract version of
-`../common/UCBasicTypes.ec`, in which `port` is an abstract type.
+The file `UCBasicTypes.ec` is a stripped down, more abstract version
+of `../common/UCBasicTypes.ec`, in which `port` is an abstract type.
